\chapter{Signs}

$w({V_{{\bf{e}}_j}^i})=\frac 1 N$

\begin{equation}
\begin{aligned}
{\color{blue}w(}&{\color{blue}{\tilde{V}}_{{\bf{e}}_m})}
= \frac
{S({\bf{g}} \to {{\tilde{V}}_{{\bf{e}}_m}}) }
{\sum\limits^N_{i=1}{ S({\bf{g}} \to {V^i_{{{\bf{e}}_m}}})}  }\\
&
\begin{aligned}
= \frac
{ \sum\limits_{{{\bf{e}}_j} \in {\bf{g}}- \{ {{\bf{e}}_m} \}} {
\sum\limits^N_{k=1} {S({{V^k_{{{\bf{e}}_j}}} \to {{\tilde{V}}_{{{\bf{e}}_m}}}})\color{blue}{w(V^k_{{\bf{e}}_j})}}
}   }
{\sum\limits^N_{i=1}{
\sum\limits_{{{\bf{e}}_j} \in {\bf{g}}- \{ {{\bf{e}}_m} \}} {
\sum\limits^N_{k=1} {S({{V^k_{{{\bf{e}}_j}}} \to {V^i_{{{\bf{e}}_m}}}})\color{blue}{w(V^k_{{\bf{e}}_j})}}
}
}  }\:.
\end{aligned}
\end{aligned}
\label{eq4}
\end{equation}

\[
{\bf{p}}=[F_{\bf{p}}^1,F_{\bf{p}}^2,...,F_{\bf{p}}^{d},\frac {x_{\bf{p}}} {w_I} , \frac {y_{\bf{p}}} {h_I}]\ .
\]

\begin{equation}
\label{eq:pms4}
\omega_{g(i,j)}=\sqrt{ (d\times{2^i})\times(2 \times {2^j})  }.
\end{equation}
